wip: generalize p256 to also work on 32-bit platforms

code/ecdsap256/Hacl.Impl.P256.Bignum.fst
@@ -15,38 +15,48 @@ module LSeq = Lib.Sequence
 
 #set-options "--z3rlimit 50 --fuel 0 --ifuel 0"
 
-let bn_v_is_as_nat a =
-  let open Lib.Sequence in
-  let open Hacl.Spec.Bignum.Definitions in
-  assert_norm (pow2 64 * pow2 64 = pow2 128);
-  assert_norm (pow2 64 * pow2 64 * pow2 64 = pow2 192);
-
-  calc (==) {
-    bn_v a;
-  (==) { bn_eval1 (slice a 0 1); bn_eval_split_i #U64 a 1 }
-    v a.[0] + pow2 64 * bn_v (slice a 1 4);
-  (==) { bn_eval_split_i #U64 (slice a 1 4) 1; bn_eval1 (slice a 1 2) }
-    v a.[0] + pow2 64 * v a.[1] + pow2 64 * pow2 64 * bn_v (slice a 2 4);
-  (==) { bn_eval_split_i #U64 (slice a 2 4) 1; bn_eval1 (slice a 2 3) }
-    v a.[0] + pow2 64 * v a.[1] + pow2 64 * pow2 64 * v a.[2]
-    + pow2 64 * pow2 64 * pow2 64 * bn_v (slice a 3 4);
-  (==) { bn_eval1 (slice a 3 4) }
-    v a.[0] + pow2 64 * v a.[1] + pow2 64 * pow2 64 * v a.[2]
-    + pow2 64 * pow2 64 * pow2 64 * v a.[3];
-  }
+val bn_v_is_as_nat: #l:BD.limb_t -> a:LSeq.lseq (BD.limb l) (v (nlimbs l)) ->
+  Lemma (
+    match l with
+    | U64 -> 
+          let (s0, s1, s2, s3) = LSeq.(a.[0], a.[1], a.[2], a.[3]) in
+          BD.bn_v a == v s0 + v s1 * pow2 64 + v s2 * pow2 128 + v s3 * pow2 192
+    | U32 ->
+          let (s0, s1, s2, s3, s4, s5, s6, s7) =
+          LSeq.(a.[0], a.[1], a.[2], a.[3], a.[4], a.[5], a.[6], a.[7]) in
+          BD.bn_v a == v s0 + v s1 * pow2 32 + v s2 * pow2 64 + v s3 * pow2 96 +  v s4 * pow2 128 + v s5 * pow2 160 + v s6 * pow2 192 + v s7 * pow2 224)
 
 
-///  Create a bignum
+let bn_v_is_as_nat #l a =
+  match l with
+  | U64 -> 
+    let a : LSeq.lseq uint64 4 = a in
+    let open Lib.Sequence in
+    let open Hacl.Spec.Bignum.Definitions in
+    assert_norm (pow2 64 * pow2 64 = pow2 128);
+    assert_norm (pow2 64 * pow2 64 * pow2 64 = pow2 192);
 
-let create_felem () =
-  BD.bn_eval_zeroes #U64 4 4;
-  create 4ul (u64 0)
+    calc (==) {
+      bn_v a;
+    (==) { bn_eval1 (slice a 0 1); bn_eval_split_i #U64 a 1 }
+      v a.[0] + pow2 64 * bn_v (slice a 1 4);
+    (==) { bn_eval_split_i #U64 (slice a 1 4) 1; bn_eval1 (slice a 1 2) }
+      v a.[0] + pow2 64 * v a.[1] + pow2 64 * pow2 64 * bn_v (slice a 2 4);
+    (==) { bn_eval_split_i #U64 (slice a 2 4) 1; bn_eval1 (slice a 2 3) }
+      v a.[0] + pow2 64 * v a.[1] + pow2 64 * pow2 64 * v a.[2]
+      + pow2 64 * pow2 64 * pow2 64 * bn_v (slice a 3 4);
+    (==) { bn_eval1 (slice a 3 4) }
+      v a.[0] + pow2 64 * v a.[1] + pow2 64 * pow2 64 * v a.[2]
+      + pow2 64 * pow2 64 * pow2 64 * v a.[3];
+    }
+  | U32 -> admit()
 
 
-let create_widefelem () =
-  BD.bn_eval_zeroes #U64 8 8;
-  create 8ul (u64 0)
-
+inline_for_extraction noextract
+val bn_make_u64_4: res:felem U64 -> a0:uint64 -> a1:uint64 -> a2:uint64 -> a3:uint64 -> Stack unit
+  (requires fun h -> live h res)
+  (ensures  fun h0 _ h1 -> modifies (loc res) h0 h1 /\
+    as_nat h1 res = v a0 + v a1 * pow2 64 + v a2 * pow2 128 + v a3 * pow2 192)
 
 let bn_make_u64_4 res a0 a1 a2 a3 =
   let h0 = ST.get () in
@@ -65,135 +75,189 @@ let bn_make_u64_4 res a0 a1 a2 a3 =
   bn_v_is_as_nat (as_seq h0 res)
 
 
+inline_for_extraction noextract
+val bn_make_u32_8: res:felem U32 -> a0:uint32 -> a1:uint32 -> a2:uint32 -> a3:uint32 -> a4:uint32 -> a5:uint32 -> a6:uint32 -> a7:uint32 -> Stack unit
+  (requires fun h -> live h res)
+  (ensures  fun h0 _ h1 -> modifies (loc res) h0 h1 /\
+    as_nat h1 res = v a0 + v a1 * pow2 32 + v a2 * pow2 64 + v a3 * pow2 96 +  v a4 * pow2 128 + v a5 * pow2 160 + v a6 * pow2 192 + v a7 * pow2 224)
+
+let bn_make_u32_8 res a0 a1 a2 a3 a4 a5 a6 a7 =
+  let h0 = ST.get () in
+  upd res 0ul a0;
+  let h1 = ST.get () in
+  upd res 1ul a1;
+  let h2 = ST.get () in
+  upd res 2ul a2;
+  let h3 = ST.get () in
+  upd res 3ul a3;
+  let h4 = ST.get () in
+  upd res 4ul a4;
+  let h5 = ST.get () in
+  upd res 5ul a5;
+  let h6 = ST.get () in
+  upd res 6ul a6;
+  let h7 = ST.get () in
+  upd res 7ul a7;
+  let h8 = ST.get () in
+  BD.bn_upd_eval (as_seq h0 res) a0 0;
+  BD.bn_upd_eval (as_seq h1 res) a1 1;
+  BD.bn_upd_eval (as_seq h2 res) a2 2;
+  BD.bn_upd_eval (as_seq h3 res) a3 3;
+  BD.bn_upd_eval (as_seq h4 res) a3 4;
+  BD.bn_upd_eval (as_seq h5 res) a3 5;
+  BD.bn_upd_eval (as_seq h6 res) a3 6;
+  BD.bn_upd_eval (as_seq h7 res) a3 3;
+  bn_v_is_as_nat (as_seq h0 res);
+  admit()
+
+let felem_make_u64_4 #l res a0 a1 a2 a3 =
+  admit();
+  bn_make_u64_4 res a0 a1 a2 a3
+  
+///  Create a bignum
+
+let create_felem l =
+  BD.bn_eval_zeroes #l (v (nlimbs l)) (v (nlimbs l));
+  create (nlimbs l) (limb_zero l)
+
+let create_widefelem l =
+  BD.bn_eval_zeroes #l (2 * v (nlimbs l)) (2 * v (nlimbs l));
+  create (2ul *. nlimbs l) (limb_zero l)
+
+
 ///  Create zero and one
 
-let bn_set_zero4 f =
-  bn_make_u64_4 f (u64 0) (u64 0) (u64 0) (u64 0)
+let felem_set_zero #l f =
+  match l with
+  | U64 -> bn_make_u64_4 f (u64 0) (u64 0) (u64 0) (u64 0)
+  | U32 -> bn_make_u32_8 f (u32 0) (u32 0) (u32 0) (u32 0) (u32 0) (u32 0) (u32 0) (u32 0)
 
 
-let bn_set_one4 f =
-  bn_make_u64_4 f (u64 1) (u64 0) (u64 0) (u64 0)
-
+let felem_set_one #l f =
+  match l with
+  | U64 -> bn_make_u64_4 f (u64 1) (u64 0) (u64 0) (u64 0)
+  | U32 -> bn_make_u32_8 f (u32 1) (u32 0) (u32 0) (u32 0) (u32 0) (u32 0) (u32 0) (u32 0)
 
 ///  Comparison
 
 [@CInline]
-let bn_is_zero_mask4 f =
+let felem_is_zero_mask #l f =
   let h0 = ST.get () in
   SN.bn_is_zero_mask_lemma (as_seq h0 f);
-  bn_v_is_as_nat (as_seq h0 f);
-  BN.bn_is_zero_mask #U64 4ul f
+  bn_v_is_as_nat #l (as_seq h0 f);
+  BN.bn_is_zero_mask #l (nlimbs l) f
 
 
 [@CInline]
-let bn_is_zero_vartime4 f =
-  let m = bn_is_zero_mask4 f in
+let felem_is_zero_vartime f =
+  let m = felem_is_zero_mask f in
   Hacl.Bignum.Base.unsafe_bool_of_limb m
 
 
 [@CInline]
-let bn_is_eq_mask4 a b =
+let felem_is_eq_mask #l a b =
   let h0 = ST.get () in
   SN.bn_eq_mask_lemma (as_seq h0 a) (as_seq h0 b);
-  bn_v_is_as_nat (as_seq h0 a);
-  bn_v_is_as_nat (as_seq h0 b);
-  BN.bn_eq_mask #U64 4ul a b
-
+  bn_v_is_as_nat #l (as_seq h0 a);
+  bn_v_is_as_nat #l (as_seq h0 b);
+  admit();
+  BN.bn_eq_mask #l (nlimbs l) a b
+  
 
 [@CInline]
-let bn_is_eq_vartime4 a b =
-  let m = bn_is_eq_mask4 a b in
+let felem_is_eq_vartime a b =
+  let m = felem_is_eq_mask a b in
   Hacl.Bignum.Base.unsafe_bool_of_limb m
 
 
-let bn_is_odd4 f =
+let felem_is_odd #l f =
   let h0 = ST.get () in
   bn_v_is_as_nat (as_seq h0 f);
   SN.bn_is_odd_lemma (as_seq h0 f);
-  BN.bn_is_odd 4ul f
+  BN.bn_is_odd (nlimbs l) f
 
 
 ///  Conditional copy
 
 [@CInline]
-let bn_cmovznz4 res cin x y =
-  let mask = neq_mask cin (u64 0) in
+let felem_cmovznz #l res cin x y =
+  let mask = neq_mask cin (limb_zero l) in
   Lib.ByteBuffer.buf_mask_select y x mask res
 
 
 ///  Addition and subtraction
 
 [@CInline]
-let bn_add_mod4 res n x y =
+let felem_add_mod #l res n x y =
   let h0 = ST.get () in
   SN.bn_add_mod_n_lemma (as_seq h0 n) (as_seq h0 x) (as_seq h0 y);
-  BN.bn_add_mod_n 4ul n x y res
+  BN.bn_add_mod_n (nlimbs l) n x y res
 
 
 [@CInline]
-let bn_sub4 res x y =
+let felem_sub #l res x y =
   let h0 = ST.get () in
   SN.bn_sub_lemma (as_seq h0 x) (as_seq h0 y);
-  let c = BN.bn_sub_eq_len 4ul x y res in
+  let c = BN.bn_sub_eq_len (nlimbs l) x y res in
   let h1 = ST.get () in
   assert (as_nat h1 res - v c * pow2 256 = as_nat h0 x - as_nat h0 y);
-  BD.bn_eval_bound (as_seq h1 res) 4;
-  BD.bn_eval_bound (as_seq h0 x) 4;
-  BD.bn_eval_bound (as_seq h0 y) 4;
+  BD.bn_eval_bound (as_seq h1 res) (v (nlimbs l));
+  BD.bn_eval_bound (as_seq h0 x) (v (nlimbs l));
+  BD.bn_eval_bound (as_seq h0 y) (v (nlimbs l));
   assert (if v c = 0 then as_nat h0 x >= as_nat h0 y else as_nat h0 x < as_nat h0 y);
   c
 
 
 [@CInline]
-let bn_sub_mod4 res n x y =
+let felem_sub_mod #l res n x y =
   let h0 = ST.get () in
   SN.bn_sub_mod_n_lemma (as_seq h0 n) (as_seq h0 x) (as_seq h0 y);
-  BN.bn_sub_mod_n 4ul n x y res
+  BN.bn_sub_mod_n (nlimbs l) n x y res
 
 
 ///  Multiplication
 
 [@CInline]
-let bn_mul4 res x y =
+let felem_mul #l res x y =
   let h0 = ST.get () in
   SN.bn_mul_lemma (as_seq h0 x) (as_seq h0 y);
-  BN.bn_mul #U64 4ul 4ul x y res
+  BN.bn_mul #l (nlimbs l) (nlimbs l) x y res
 
 
 [@CInline]
-let bn_sqr4 res x =
+let felem_sqr #l res x =
   let h0 = ST.get () in
   SN.bn_sqr_lemma (as_seq h0 x);
-  BN.bn_sqr #U64 4ul x res
+  BN.bn_sqr #l (nlimbs l) x res
 
 
 ///  Conversion between bignum and bytes representation
 
 [@CInline]
-let bn_to_bytes_be4 res f =
+let felem_to_bytes_be #l res f =
   let h0 = ST.get () in
-  Hacl.Spec.Bignum.Convert.bn_to_bytes_be_lemma #U64 32 (as_seq h0 f);
+  Hacl.Spec.Bignum.Convert.bn_to_bytes_be_lemma #l 32 (as_seq h0 f);
   Hacl.Bignum.Convert.mk_bn_to_bytes_be true 32ul f res
 
 
 [@CInline]
-let bn_from_bytes_be4 res b =
+let felem_from_bytes_be #l res b =
   let h0 = ST.get () in
-  Hacl.Spec.Bignum.Convert.bn_from_bytes_be_lemma #U64 32 (as_seq h0 b);
+  Hacl.Spec.Bignum.Convert.bn_from_bytes_be_lemma #l 32 (as_seq h0 b);
   Hacl.Bignum.Convert.mk_bn_from_bytes_be true 32ul b res
 
 
 [@CInline]
-let bn2_to_bytes_be4 res x y =
+let felem2_to_bytes_be res x y =
   let h0 = ST.get () in
   update_sub_f h0 res 0ul 32ul
     (fun h -> BSeq.nat_to_bytes_be 32 (as_nat h0 x))
-    (fun _ -> bn_to_bytes_be4 (sub res 0ul 32ul) x);
+    (fun _ -> felem_to_bytes_be (sub res 0ul 32ul) x);
 
   let h1 = ST.get () in
   update_sub_f h1 res 32ul 32ul
     (fun h -> BSeq.nat_to_bytes_be 32 (as_nat h1 y))
-    (fun _ -> bn_to_bytes_be4 (sub res 32ul 32ul) y);
+    (fun _ -> felem_to_bytes_be (sub res 32ul 32ul) y);
 
   let h2 = ST.get () in
   let x = Ghost.hide (BSeq.nat_to_bytes_be 32 (as_nat h0 x)) in
