code/ecdsap256/Hacl.Impl.P256.Bignum.fsti
@@ -14,59 +14,78 @@ module BD = Hacl.Spec.Bignum.Definitions
 
 #set-options "--z3rlimit 50 --fuel 0 --ifuel 0"
 
+let limb_t = BD.limb_t
+let limb l = BD.limb l
+
+[@@strict_on_arguments [0]]
+unfold
+let limb_zero l : BD.limb l =
+  match l with
+  | U64 -> u64 0
+  | U32 -> u32 0
+
+[@@strict_on_arguments [0]]
+unfold
+let limb_one l : BD.limb l =
+  match l with
+  | U64 -> u64 1
+  | U32 -> u32 1
+
+[@@strict_on_arguments [0]]
+unfold
+let nlimbs (l:limb_t) =
+  match l with
+  | U64 -> 4ul
+  | U32 -> 8ul
+
 inline_for_extraction
-let felem = lbuffer uint64 (size 4)
+let felem (l:limb_t) = lbuffer (limb l) (nlimbs l)
 inline_for_extraction
-let widefelem = lbuffer uint64 (size 8)
+let widefelem (l:limb_t) = lbuffer (limb l) (2ul *. nlimbs l)
 
 unfold
-let as_nat (h:mem) (e:felem) : GTot nat =
+let as_nat #l (h:mem) (e:felem l) : GTot nat =
   BD.bn_v (as_seq h e)
 
 unfold
-let wide_as_nat (h:mem) (e:widefelem) : GTot nat =
+let wide_as_nat #l (h:mem) (e:widefelem l) : GTot nat =
   BD.bn_v (as_seq h e)
-
-val bn_v_is_as_nat: a:LSeq.lseq uint64 4 ->
-  Lemma (let (s0, s1, s2, s3) = LSeq.(a.[0], a.[1], a.[2], a.[3]) in
-    BD.bn_v a == v s0 + v s1 * pow2 64 + v s2 * pow2 128 + v s3 * pow2 192)
 
 ///  Create a bignum
 
 inline_for_extraction noextract
-val create_felem: unit -> StackInline felem
+val felem_make_u64_4: #l:limb_t -> res:felem l -> a0:uint64 -> a1:uint64 -> a2:uint64 -> a3:uint64 -> Stack unit
+  (requires fun h -> live h res)
+  (ensures  fun h0 _ h1 -> modifies (loc res) h0 h1 /\
+    as_nat h1 res = v a0 + v a1 * pow2 64 + v a2 * pow2 128 + v a3 * pow2 192)
+
+inline_for_extraction noextract
+val create_felem: l:limb_t -> StackInline (felem l)
   (requires fun h -> True)
   (ensures  fun h0 f h1 ->
-    stack_allocated f h0 h1 (LSeq.create 4 (u64 0)) /\
+    stack_allocated f h0 h1 (LSeq.create (v (nlimbs l)) (uint #l 0)) /\
     as_nat h1 f == 0)
 
 
 inline_for_extraction noextract
-val create_widefelem: unit -> StackInline widefelem
+val create_widefelem: l:limb_t -> StackInline (widefelem l)
   (requires fun h -> True)
   (ensures  fun h0 f h1 ->
-    stack_allocated f h0 h1 (LSeq.create 8 (u64 0)) /\
+    stack_allocated f h0 h1 (LSeq.create (v (2ul *. nlimbs l)) (uint #l 0)) /\
     wide_as_nat h1 f == 0)
-
-
-inline_for_extraction noextract
-val bn_make_u64_4: res:felem -> a0:uint64 -> a1:uint64 -> a2:uint64 -> a3:uint64 -> Stack unit
-  (requires fun h -> live h res)
-  (ensures  fun h0 _ h1 -> modifies (loc res) h0 h1 /\
-    as_nat h1 res = v a0 + v a1 * pow2 64 + v a2 * pow2 128 + v a3 * pow2 192)
 
 
 ///  Create zero and one
 
 inline_for_extraction noextract
-val bn_set_zero4: f:felem -> Stack unit
+val felem_set_zero: #l:limb_t -> f:felem l -> Stack unit
   (requires fun h -> live h f)
   (ensures fun h0 _ h1 -> modifies (loc f) h0 h1 /\
     as_nat h1 f == 0)
 
 
 inline_for_extraction noextract
-val bn_set_one4: f:felem -> Stack unit
+val felem_set_one: #l:limb_t -> f:felem l -> Stack unit
   (requires fun h -> live h f)
   (ensures fun h0 _ h1 -> modifies (loc f) h0 h1 /\
     as_nat h1 f == 1)
@@ -74,31 +93,31 @@ val bn_set_one4: f:felem -> Stack unit
 
 ///  Comparison
 
-val bn_is_zero_mask4: f:felem -> Stack uint64
+val felem_is_zero_mask: #l:limb_t -> f:felem l -> Stack (limb l)
   (requires fun h -> live h f)
   (ensures fun h0 r h1 -> modifies0 h0 h1 /\
-    (if as_nat h0 f = 0 then v r == ones_v U64 else v r == 0))
+    (if as_nat h0 f = 0 then v r == ones_v l else v r == 0))
 
 
-val bn_is_zero_vartime4: f:felem -> Stack bool
+val felem_is_zero_vartime: #l:limb_t -> f:felem l -> Stack bool
   (requires fun h -> live h f)
   (ensures fun h0 r h1 -> modifies0 h0 h1 /\ r == (as_nat h0 f = 0))
 
 
-val bn_is_eq_mask4: x:felem -> y:felem -> Stack uint64
+val felem_is_eq_mask: #l:limb_t -> x:felem l -> y:felem l -> Stack (limb l)
   (requires fun h -> live h x /\ live h y)
   (ensures fun h0 r h1 -> modifies0 h0 h1 /\
     (if as_nat h0 x = as_nat h0 y then v r == ones_v U64 else v r = 0))
 
 
-val bn_is_eq_vartime4: x:felem -> y:felem -> Stack bool
+val felem_is_eq_vartime: #l:limb_t -> x:felem l -> y:felem l -> Stack bool
   (requires fun h -> live h x /\ live h y)
   (ensures  fun h0 r h1 -> modifies0 h0 h1 /\
     r == (as_nat h0 x = as_nat h0 y))
 
 
 inline_for_extraction noextract
-val bn_is_odd4: f:felem -> Stack uint64
+val felem_is_odd: #l:limb_t -> f:felem l -> Stack (limb l)
   (requires fun h -> live h f)
   (ensures  fun h0 r h1 -> modifies0 h0 h1 /\
     v r = (as_nat h0 f % 2))
@@ -106,7 +125,7 @@ val bn_is_odd4: f:felem -> Stack uint64
 
 ///  Conditional copy
 
-val bn_cmovznz4: res:felem -> cin:uint64 -> x:felem -> y:felem -> Stack unit
+val felem_cmovznz: #l:limb_t -> res:felem l -> cin:limb l -> x:felem l -> y:felem l -> Stack unit
   (requires fun h ->
     live h x /\ live h y /\ live h res /\
     eq_or_disjoint res x /\ eq_or_disjoint res y /\ eq_or_disjoint x y)
@@ -116,7 +135,7 @@ val bn_cmovznz4: res:felem -> cin:uint64 -> x:felem -> y:felem -> Stack unit
 
 ///  Addition and subtraction
 
-val bn_add_mod4: res:felem -> n:felem -> x:felem -> y:felem -> Stack unit
+val felem_add_mod: #l:limb_t -> res:felem l -> n:felem l -> x:felem l -> y:felem l -> Stack unit
   (requires fun h ->
     live h n /\ live h x /\ live h y /\ live h res /\
     disjoint n x /\ disjoint n y /\ disjoint n res /\
@@ -126,7 +145,7 @@ val bn_add_mod4: res:felem -> n:felem -> x:felem -> y:felem -> Stack unit
     as_nat h1 res == (as_nat h0 x + as_nat h0 y) % as_nat h0 n)
 
 
-val bn_sub4: res:felem -> x:felem -> y:felem -> Stack uint64
+val felem_sub: #l:limb_t -> res:felem l -> x:felem l -> y:felem l -> Stack (limb l)
   (requires fun h ->
     live h x /\ live h y /\ live h res /\
     eq_or_disjoint x y /\ eq_or_disjoint x res /\ eq_or_disjoint y res)
@@ -135,7 +154,7 @@ val bn_sub4: res:felem -> x:felem -> y:felem -> Stack uint64
     (if v c = 0 then as_nat h0 x >= as_nat h0 y else as_nat h0 x < as_nat h0 y))
 
 
-val bn_sub_mod4: res:felem -> n:felem -> x:felem -> y:felem -> Stack unit
+val felem_sub_mod: #l:limb_t -> res:felem l -> n:felem l -> x:felem l -> y:felem l -> Stack unit
   (requires fun h ->
     live h n /\ live h x /\ live h y /\ live h res /\
     disjoint n x /\ disjoint n y /\ disjoint n res /\
@@ -147,7 +166,7 @@ val bn_sub_mod4: res:felem -> n:felem -> x:felem -> y:felem -> Stack unit
 
 ///  Multiplication
 
-val bn_mul4: res:widefelem -> x:felem -> y:felem -> Stack unit
+val felem_mul: #l:limb_t -> res:widefelem l -> x:felem l -> y:felem l -> Stack unit
   (requires fun h ->
     live h res /\ live h x /\ live h y /\
     eq_or_disjoint x y /\ disjoint x res /\ disjoint y res)
@@ -155,7 +174,7 @@ val bn_mul4: res:widefelem -> x:felem -> y:felem -> Stack unit
     wide_as_nat h1 res = as_nat h0 x * as_nat h0 y)
 
 
-val bn_sqr4: res:widefelem -> x:felem -> Stack unit
+val felem_sqr: #l:limb_t -> res:widefelem l -> x:felem l -> Stack unit
   (requires fun h ->
     live h res /\ live h x /\ eq_or_disjoint x res)
   (ensures  fun h0 _ h1 -> modifies (loc res) h0 h1 /\
@@ -164,7 +183,7 @@ val bn_sqr4: res:widefelem -> x:felem -> Stack unit
 
 ///  Conversion between bignum and bytes representation
 
-val bn_to_bytes_be4: res:lbuffer uint8 32ul -> f:felem -> Stack unit
+val felem_to_bytes_be: #l:limb_t -> res:lbuffer uint8 32ul -> f:felem l -> Stack unit
   (requires fun h ->
     live h f /\ live h res /\ disjoint f res /\
     as_nat h f < pow2 256)
@@ -172,13 +191,13 @@ val bn_to_bytes_be4: res:lbuffer uint8 32ul -> f:felem -> Stack unit
     as_seq h1 res == BSeq.nat_to_bytes_be 32 (as_nat h0 f))
 
 
-val bn_from_bytes_be4: res:felem -> b:lbuffer uint8 32ul -> Stack unit
+val felem_from_bytes_be: #l:limb_t -> res:felem l -> b:lbuffer uint8 32ul -> Stack unit
   (requires fun h -> live h b /\ live h res /\ disjoint b res)
   (ensures  fun h0 _ h1 -> modifies (loc res) h0 h1 /\
     as_nat h1 res == BSeq.nat_from_bytes_be (as_seq h0 b))
 
 
-val bn2_to_bytes_be4: res:lbuffer uint8 64ul -> x:felem -> y:felem -> Stack unit
+val felem2_to_bytes_be: #l:limb_t -> res:lbuffer uint8 64ul -> x:felem l -> y:felem l -> Stack unit
   (requires fun h ->
     live h x /\ live h y /\ live h res /\
     disjoint x res /\ disjoint y res /\
@@ -186,3 +205,4 @@ val bn2_to_bytes_be4: res:lbuffer uint8 64ul -> x:felem -> y:felem -> Stack unit
   (ensures fun h0 _ h1 -> modifies (loc res) h0 h1 /\
     as_seq h1 res == LSeq.concat #uint8 #32 #32
       (BSeq.nat_to_bytes_be 32 (as_nat h0 x)) (BSeq.nat_to_bytes_be 32 (as_nat h0 y)))
+
