code/ecdsap256/Hacl.Impl.P256.Field.fsti
@@ -15,19 +15,19 @@ module SM = Hacl.Spec.P256.Montgomery
 
 #set-options "--z3rlimit 50 --fuel 0 --ifuel 0"
 
-let fmont_as_nat (h:mem) (a:felem) = SM.from_mont (as_nat h a)
+let fmont_as_nat #l (h:mem) (a:felem l) = SM.from_mont (as_nat h a)
 
 
 ///  Create zero and one
 
-val make_fzero: n:felem -> Stack unit
+val make_fzero: #l:limb_t -> n:felem l -> Stack unit
   (requires fun h -> live h n)
   (ensures  fun h0 _ h1 -> modifies (loc n) h0 h1 /\
     as_nat h1 n < S.prime /\
     fmont_as_nat h1 n == 0)
 
 
-val make_fone: n:felem -> Stack unit
+val make_fone: #l:limb_t -> n:felem l -> Stack unit
   (requires fun h -> live h n)
   (ensures  fun h0 _ h1 -> modifies (loc n) h0 h1 /\
     as_nat h1 n < S.prime /\
@@ -36,13 +36,13 @@ val make_fone: n:felem -> Stack unit
 
 ///  Comparison
 
-val bn_is_lt_prime_mask4: f:felem -> Stack uint64
+val felem_is_lt_prime_mask: #l:limb_t -> f:felem l -> Stack (limb l)
   (requires fun h -> live h f)
   (ensures  fun h0 r h1 -> modifies0 h0 h1 /\
     (if as_nat h0 f < S.prime then v r = ones_v U64 else v r = 0))
 
 
-val feq_mask: a:felem -> b:felem -> Stack uint64
+val feq_mask: #l:limb_t -> a:felem l -> b:felem l -> Stack (limb l)
   (requires fun h ->
     live h a /\ live h b /\ eq_or_disjoint a b /\
     as_nat h a < S.prime /\ as_nat h b < S.prime)
@@ -52,7 +52,7 @@ val feq_mask: a:felem -> b:felem -> Stack uint64
 
 ///  Field Arithmetic
 
-val fadd: res:felem -> x:felem -> y:felem -> Stack unit
+val fadd: #l:limb_t -> res:felem l -> x:felem l -> y:felem l -> Stack unit
   (requires fun h ->
     live h x /\ live h y /\ live h res /\
     eq_or_disjoint x y /\ eq_or_disjoint x res /\ eq_or_disjoint y res /\
@@ -63,7 +63,7 @@ val fadd: res:felem -> x:felem -> y:felem -> Stack unit
 
 
 inline_for_extraction noextract
-val fdouble: res:felem -> x:felem -> Stack unit
+val fdouble: #l:limb_t -> res:felem l -> x:felem l -> Stack unit
   (requires fun h ->
     live h x /\ live h res /\ eq_or_disjoint x res /\
     as_nat h x < S.prime)
@@ -72,7 +72,7 @@ val fdouble: res:felem -> x:felem -> Stack unit
     fmont_as_nat h1 res == (2 * fmont_as_nat h0 x) % S.prime)
 
 
-val fsub: res:felem -> x:felem -> y:felem -> Stack unit
+val fsub: #l:limb_t -> res:felem l -> x:felem l -> y:felem l -> Stack unit
   (requires fun h ->
     live h res /\ live h x /\ live h y /\
     eq_or_disjoint x y /\ eq_or_disjoint x res /\ eq_or_disjoint y res /\
@@ -82,13 +82,13 @@ val fsub: res:felem -> x:felem -> y:felem -> Stack unit
     fmont_as_nat h1 res == S.fsub (fmont_as_nat h0 x) (fmont_as_nat h0 y))
 
 
-val fnegate_conditional_vartime: f:felem -> is_negate:bool -> Stack unit
+val fnegate_conditional_vartime: #l:limb_t -> f:felem l -> is_negate:bool -> Stack unit
   (requires fun h -> live h f /\ as_nat h f < S.prime)
   (ensures  fun h0 _ h1 -> modifies (loc f) h0 h1 /\ as_nat h1 f < S.prime /\
     as_nat h1 f == (if is_negate then (S.prime - as_nat h0 f) % S.prime else as_nat h0 f))
 
 
-val fmul: res:felem -> x:felem -> y:felem -> Stack unit
+val fmul: #l:limb_t -> res:felem l -> x:felem l -> y:felem l -> Stack unit
   (requires fun h ->
     live h x /\ live h y /\ live h res /\
     eq_or_disjoint x y /\ eq_or_disjoint x res /\ eq_or_disjoint y res /\
@@ -98,7 +98,7 @@ val fmul: res:felem -> x:felem -> y:felem -> Stack unit
     fmont_as_nat h1 res = S.fmul (fmont_as_nat h0 x) (fmont_as_nat h0 y))
 
 
-val fsqr: res:felem -> x:felem -> Stack unit
+val fsqr: #l:limb_t -> res:felem l -> x:felem l -> Stack unit
   (requires fun h ->
     live h x /\ live h res /\ eq_or_disjoint x res /\
     as_nat h x < S.prime)
@@ -107,7 +107,7 @@ val fsqr: res:felem -> x:felem -> Stack unit
     fmont_as_nat h1 res = S.fmul (fmont_as_nat h0 x) (fmont_as_nat h0 x))
 
 
-val from_mont: res:felem -> x:felem -> Stack unit
+val from_mont: #l:limb_t -> res:felem l -> x:felem l -> Stack unit
   (requires fun h ->
     live h x /\ live h res /\ as_nat h x < S.prime)
   (ensures  fun h0 _ h1 -> modifies (loc res) h0 h1 /\
@@ -115,7 +115,7 @@ val from_mont: res:felem -> x:felem -> Stack unit
     as_nat h1 res = fmont_as_nat h0 x)
 
 
-val to_mont: res:felem -> f:felem -> Stack unit
+val to_mont: #l:limb_t -> res:felem l -> f:felem l -> Stack unit
   (requires fun h ->
     live h f /\ live h res /\ eq_or_disjoint f res /\
     as_nat h f < S.prime)
@@ -125,7 +125,7 @@ val to_mont: res:felem -> f:felem -> Stack unit
 
 ///  Special cases of the above functions
 
-val fmul_by_b_coeff: res:felem -> x:felem -> Stack unit
+val fmul_by_b_coeff: #l:limb_t -> res:felem l -> x:felem l -> Stack unit
   (requires fun h ->
     live h x /\ live h res /\ eq_or_disjoint x res /\
     as_nat h x < S.prime)
@@ -135,7 +135,7 @@ val fmul_by_b_coeff: res:felem -> x:felem -> Stack unit
       S.fmul S.b_coeff (fmont_as_nat h0 x))
 
 
-val fcube: res:felem -> x:felem -> Stack unit
+val fcube: #l:limb_t -> res:felem l  -> x:felem l -> Stack unit
   (requires fun h ->
     live h x /\ live h res /\ disjoint x res /\
     as_nat h x < S.prime)
