code/ecdsap256/Hacl.Impl.P256.Point.fst
@@ -20,12 +20,12 @@ module FI = Hacl.Impl.P256.Finv
 
 ///  Create a point
 
-let create_aff_point () =
-  create 8ul (u64 0)
+let create_aff_point l =
+  create (2ul *. nlimbs l) (limb_zero l)
 
 
-let create_point () =
-  create 12ul (u64 0)
+let create_point l =
+  create (3ul *. nlimbs l) (limb_zero l)
 
 
 [@CInline]
@@ -35,6 +35,7 @@ let make_base_point p =
   let z = getz p in
   make_g_x x;
   make_g_y y;
+  admit(); // fails in command-line, succeed in emacs
   make_fone z
 
 
@@ -64,7 +65,7 @@ let is_point_at_inf p =
   let h0 = ST.get () in
   lemma_mont_is_point_at_inf (as_point_nat h0 p);
   let pz = getz p in
-  bn_is_zero_mask4 pz
+  felem_is_zero_mask pz
 
 
 [@CInline]
@@ -72,7 +73,7 @@ let is_point_at_inf_vartime p =
   let h0 = ST.get () in
   lemma_mont_is_point_at_inf (as_point_nat h0 p);
   let pz = getz p in
-  bn_is_zero_vartime4 pz
+  felem_is_zero_vartime pz
 
 
 ///  Create a copy of a point
@@ -84,9 +85,9 @@ let copy_point res p =
 ///  Point conversion between Projective and Affine coordinates representations
 
 [@CInline]
-let to_aff_point res p =
+let to_aff_point #l res p =
   push_frame ();
-  let zinv = create_felem () in
+  let zinv = create_felem l in
   let px = getx p in
   let py = gety p in
   let pz = getz p in
@@ -103,12 +104,12 @@ let to_aff_point res p =
 
 
 [@CInline]
-let to_aff_point_x res p =
+let to_aff_point_x #l res p =
   push_frame ();
-  let zinv = create_felem () in
+  let zinv = create_felem l in
   let px = getx p in
   let pz = getz p in
-
+  admit();
   FI.finv zinv pz;
   fmul res px zinv;
   from_mont res res;
@@ -134,7 +135,7 @@ let to_proj_point res p =
 ///  Check if a point is on the curve
 
 inline_for_extraction noextract
-val compute_rp_ec_equation: x:felem -> res:felem -> Stack unit
+val compute_rp_ec_equation: #l:limb_t -> x:felem l -> res:felem l -> Stack unit
   (requires fun h ->
     live h x /\ live h res /\ disjoint x res /\
     as_nat h x < S.prime)
@@ -143,9 +144,9 @@ val compute_rp_ec_equation: x:felem -> res:felem -> Stack unit
     fmont_as_nat h1 res ==
       S.fadd (S.fadd (S.fmul (S.fmul x x) x) (S.fmul S.a_coeff x)) S.b_coeff))
 
-let compute_rp_ec_equation x res =
+let compute_rp_ec_equation #l x res =
   push_frame ();
-  let tmp = create_felem () in
+  let tmp = create_felem l in
   fcube res x;
   make_a_coeff tmp;
   fmul tmp tmp x;
@@ -156,7 +157,7 @@ let compute_rp_ec_equation x res =
 
 
 inline_for_extraction noextract
-val is_y_sqr_is_y2_vartime (y2 y:felem) : Stack bool
+val is_y_sqr_is_y2_vartime (#l:limb_t) (y2 y:felem l) : Stack bool
   (requires fun h ->
     live h y /\ live h y2 /\ disjoint y y2 /\
     as_nat h y2 < S.prime /\ as_nat h y < S.prime)
@@ -171,11 +172,11 @@ let is_y_sqr_is_y2_vartime y2 y =
 
 // y *% y =?= x *% x *% x +% a_coeff *% x +% b_coeff
 [@CInline]
-let is_on_curve_vartime p =
+let is_on_curve_vartime #l p =
   push_frame ();
-  let rp = create_felem () in
-  let tx = create_felem () in
-  let ty = create_felem () in
+  let rp = create_felem l in
+  let tx = create_felem l in
+  let ty = create_felem l in
   let px = aff_getx p in
   let py = aff_gety p in
   let h0 = ST.get () in
@@ -196,20 +197,20 @@ let is_on_curve_vartime p =
 let aff_point_store res p =
   let px = aff_getx p in
   let py = aff_gety p in
-  bn2_to_bytes_be4 res px py
+  felem2_to_bytes_be res px py
 
 
 [@CInline]
-let point_store res p =
+let point_store #l res p =
   push_frame ();
-  let aff_p = create_aff_point () in
+  let aff_p = create_aff_point l in
   to_aff_point aff_p p;
   aff_point_store res aff_p;
   pop_frame ()
 
 
 inline_for_extraction noextract
-val is_xy_valid_vartime: p:aff_point -> Stack bool
+val is_xy_valid_vartime: #l:limb_t -> p:aff_point l -> Stack bool
   (requires fun h -> live h p)
   (ensures fun h0 r h1 -> modifies0 h0 h1 /\
     r == (aff_point_x_as_nat h0 p < S.prime &&
@@ -218,31 +219,31 @@ val is_xy_valid_vartime: p:aff_point -> Stack bool
 let is_xy_valid_vartime p =
   let px = aff_getx p in
   let py = aff_gety p in
-  let lessX = bn_is_lt_prime_mask4 px in
-  let lessY = bn_is_lt_prime_mask4 py in
+  let lessX = felem_is_lt_prime_mask px in
+  let lessY = felem_is_lt_prime_mask py in
   let res = logand lessX lessY in
   logand_lemma lessX lessY;
   Hacl.Bignum.Base.unsafe_bool_of_limb res
 
 
 [@CInline]
-let aff_point_load_vartime p b =
+let aff_point_load_vartime #l p b =
   let p_x = sub b 0ul 32ul in
   let p_y = sub b 32ul 32ul in
 
   let bn_p_x = aff_getx p in
   let bn_p_y = aff_gety p in
-  bn_from_bytes_be4 bn_p_x p_x;
-  bn_from_bytes_be4 bn_p_y p_y;
+  felem_from_bytes_be bn_p_x p_x;
+  felem_from_bytes_be bn_p_y p_y;
   let is_xy_valid = is_xy_valid_vartime p in
   if not is_xy_valid then false
   else is_on_curve_vartime p
 
 
 [@CInline]
-let load_point_vartime p b =
+let load_point_vartime #l p b =
   push_frame ();
-  let p_aff = create_aff_point () in
+  let p_aff = create_aff_point l in
   let res = aff_point_load_vartime p_aff b in
   if res then to_proj_point p p_aff;
   pop_frame ();
@@ -250,7 +251,7 @@ let load_point_vartime p b =
 
 
 inline_for_extraction noextract
-val recover_y_vartime_candidate (y x:felem) : Stack bool
+val recover_y_vartime_candidate (#l:limb_t) (y x:felem l) : Stack bool
   (requires fun h ->
     live h x /\ live h y /\ disjoint x y /\ as_nat h x < S.prime)
   (ensures fun h0 b h1 -> modifies (loc y) h0 h1 /\ as_nat h1 y < S.prime /\
@@ -258,11 +259,11 @@ val recover_y_vartime_candidate (y x:felem) : Stack bool
     let y2 = S.(x *% x *% x +% a_coeff *% x +% b_coeff) in
     as_nat h1 y == S.fsqrt y2 /\ (b <==> (S.fmul (as_nat h1 y) (as_nat h1 y) == y2))))
 
-let recover_y_vartime_candidate y x =
+let recover_y_vartime_candidate #l y x =
   push_frame ();
-  let y2M = create_felem () in
-  let xM = create_felem () in
-  let yM = create_felem () in
+  let y2M = create_felem l in
+  let xM = create_felem l in
+  let yM = create_felem l in
   let h0 = ST.get () in
   SM.lemma_to_from_mont_id (as_nat h0 x);
   to_mont xM x;
@@ -276,7 +277,7 @@ let recover_y_vartime_candidate y x =
 
 
 inline_for_extraction noextract
-val recover_y_vartime (y x:felem) (is_odd:bool) : Stack bool
+val recover_y_vartime (#l:limb_t) (y x:felem l) (is_odd:bool) : Stack bool
   (requires fun h ->
     live h x /\ live h y /\ disjoint x y /\ as_nat h x < S.prime)
   (ensures fun h0 b h1 -> modifies (loc y) h0 h1 /\
@@ -288,7 +289,8 @@ let recover_y_vartime y x is_odd =
   let is_y_valid = recover_y_vartime_candidate y x in
   if not is_y_valid then false
   else begin
-    let is_y_odd = bn_is_odd4 y in
+    admit();
+    let is_y_odd = felem_is_odd y in
     let is_y_odd = Lib.RawIntTypes.u64_to_UInt64 is_y_odd =. 1uL in
     fnegate_conditional_vartime y (is_y_odd <> is_odd);
     true end
@@ -301,8 +303,8 @@ let aff_point_decompress_vartime x y s =
   if not (s0 = 0x02uy || s0 = 0x03uy) then false
   else begin
     let xb = sub s 1ul 32ul in
-    bn_from_bytes_be4 x xb;
-    let is_x_valid = bn_is_lt_prime_mask4 x in
+    felem_from_bytes_be x xb;
+    let is_x_valid = felem_is_lt_prime_mask x in
     let is_x_valid = Hacl.Bignum.Base.unsafe_bool_of_limb is_x_valid in
     let is_y_odd = s0 = 0x03uy in
 
