code/ecdsap256/Hacl.Impl.P256.Point.fsti
@@ -23,130 +23,131 @@ let from_mont_point (a:tuple3 nat nat nat) : S.proj_point =
 ///  Affine coordinates
 
 inline_for_extraction noextract
-let aff_point_seq = LSeq.lseq uint64 8
+let aff_point_seq l = LSeq.lseq (limb l) (2 * v (nlimbs l))
 
-let as_aff_point_nat_seq (p:aff_point_seq) =
-  BD.bn_v (LSeq.sub p 0 4),
-  BD.bn_v (LSeq.sub p 4 4)
+let as_aff_point_nat_seq #l (p:aff_point_seq l) =
+  BD.bn_v (LSeq.sub p 0 (v (nlimbs l))),
+  BD.bn_v (LSeq.sub p (v (nlimbs l)) (v (nlimbs l)))
 
-let aff_point_inv_seq (p:aff_point_seq) =
+let aff_point_inv_seq #l (p:aff_point_seq l) =
   let x, y = as_aff_point_nat_seq p in
   x < S.prime /\ y < S.prime
 
 
 inline_for_extraction noextract
-let aff_point = lbuffer uint64 8ul
+let aff_point l = lbuffer (limb l) (2ul *. nlimbs l)
 
 noextract
-let as_aff_point_nat (h:mem) (p:aff_point) =
+let as_aff_point_nat #l (h:mem) (p:aff_point l) =
   as_aff_point_nat_seq (as_seq h p)
 
 noextract
-let aff_point_inv (h:mem) (p:aff_point) =
+let aff_point_inv #l (h:mem) (p:aff_point l) =
   aff_point_inv_seq (as_seq h p)
 
 noextract
-let aff_point_x_as_nat (h:mem) (p:aff_point) : GTot nat =
-  as_nat h (gsub p 0ul 4ul)
+let aff_point_x_as_nat #l (h:mem) (p:aff_point l) : GTot nat =
+  as_nat h (gsub p 0ul (nlimbs l))
 
 noextract
-let aff_point_y_as_nat (h:mem) (p:aff_point) : GTot nat =
-  as_nat h (gsub p 4ul 4ul)
+let aff_point_y_as_nat #l (h:mem) (p:aff_point l) : GTot nat =
+  as_nat h (gsub p (nlimbs l) (nlimbs l))
 
 inline_for_extraction noextract
-let aff_getx (p:aff_point) : Stack felem
+let aff_getx #l (p:aff_point l) : Stack (felem l)
   (requires fun h -> live h p)
-  (ensures fun h0 f h1 -> f == gsub p 0ul 4ul /\ h0 == h1)
-  = sub p 0ul 4ul
+  (ensures fun h0 f h1 -> f == gsub p 0ul (nlimbs l) /\ h0 == h1)
+  = sub p 0ul (nlimbs l)
 
 inline_for_extraction noextract
-let aff_gety (p:aff_point) : Stack felem
+let aff_gety #l (p:aff_point l) : Stack (felem l)
   (requires fun h -> live h p)
-  (ensures fun h0 f h1 -> f == gsub p 4ul 4ul /\ h0 == h1)
-  = sub p 4ul 4ul
+  (ensures fun h0 f h1 -> f == gsub p (nlimbs l) (nlimbs l) /\ h0 == h1)
+  = sub p (nlimbs l) (nlimbs l)
 
 
 ///  Projective coordinates
 
 inline_for_extraction noextract
-let point_seq = LSeq.lseq uint64 12
+let point_seq (l:limb_t) = LSeq.lseq (limb l) (3 * v (nlimbs l))
 
-let as_point_nat_seq (p:point_seq) =
-  BD.bn_v (LSeq.sub p 0 4),
-  BD.bn_v (LSeq.sub p 4 4),
-  BD.bn_v (LSeq.sub p 8 4)
+let as_point_nat_seq #l (p:point_seq l) =
+  BD.bn_v (LSeq.sub p 0 (v (nlimbs l))),
+  BD.bn_v (LSeq.sub p (v (nlimbs l)) (v (nlimbs l))),
+  BD.bn_v (LSeq.sub p (2 * v (nlimbs l)) (v (nlimbs l)))
 
-let point_inv_seq (p:point_seq) =
+let point_inv_seq #l (p:point_seq l) =
   let x, y, z = as_point_nat_seq p in
   x < S.prime /\ y < S.prime /\ z < S.prime
 
 
 inline_for_extraction noextract
-let point = lbuffer uint64 12ul
+let point (l:limb_t) = lbuffer (limb l) (3ul *. nlimbs l)
 
 noextract
-let as_point_nat (h:mem) (p:point) =
+let as_point_nat #l (h:mem) (p:point l) =
   as_point_nat_seq (as_seq h p)
 
 noextract
-let point_inv (h:mem) (p:point) =
+let point_inv #l (h:mem) (p:point l) =
   point_inv_seq (as_seq h p)
 
 noextract
-let point_x_as_nat (h:mem) (p:point) : GTot nat =
-  as_nat h (gsub p 0ul 4ul)
+let point_x_as_nat #l (h:mem) (p:point l) : GTot nat =
+  as_nat h (gsub p 0ul (nlimbs l))
 
 noextract
-let point_y_as_nat (h:mem) (e:point) : GTot nat =
-  as_nat h (gsub e 4ul 4ul)
+let point_y_as_nat #l (h:mem) (e:point l) : GTot nat =
+  as_nat h (gsub e (nlimbs l) (nlimbs l))
 
 noextract
-let point_z_as_nat (h:mem) (e:point) : GTot nat =
-  as_nat h (gsub e 8ul 4ul)
+let point_z_as_nat #l (h:mem) (e:point l) : GTot nat =
+  as_nat h (gsub e (2ul *. nlimbs l) (nlimbs l))
 
 
 inline_for_extraction noextract
-let getx (p:point) : Stack felem
+let getx #l (p:point l) : Stack (felem l)
   (requires fun h -> live h p)
-  (ensures fun h0 f h1 -> f == gsub p 0ul 4ul /\ h0 == h1)
-  = sub p 0ul 4ul
+  (ensures fun h0 f h1 -> f == gsub p 0ul (nlimbs l) /\ h0 == h1)
+  = sub p 0ul (nlimbs l)
 
 inline_for_extraction noextract
-let gety (p:point) : Stack felem
+let gety #l (p:point l) : Stack (felem l)
   (requires fun h -> live h p)
-  (ensures fun h0 f h1 -> f == gsub p 4ul 4ul /\ h0 == h1)
-  = sub p 4ul 4ul
+  (ensures fun h0 f h1 -> f == gsub p (nlimbs l) (nlimbs l) /\ h0 == h1)
+  = sub p (nlimbs l) (nlimbs l)
 
 inline_for_extraction noextract
-let getz (p:point) : Stack felem
+let getz #l (p:point l) : Stack (felem l)
   (requires fun h -> live h p)
-  (ensures fun h0 f h1 -> f == gsub p 8ul 4ul /\ h0 == h1)
-  = sub p 8ul 4ul
+  (ensures fun h0 f h1 -> f == gsub p (2ul *. nlimbs l) (nlimbs l) /\ h0 == h1)
+  = sub p (2ul *. nlimbs l) (nlimbs l)
 
 
 ///  Create a point
 
 inline_for_extraction noextract
-val create_aff_point: unit -> StackInline aff_point
+val create_aff_point: l:limb_t -> StackInline (aff_point l)
   (requires fun h -> True)
   (ensures  fun h0 f h1 ->
-    stack_allocated f h0 h1 (LSeq.create 8 (u64 0)))
+    stack_allocated f h0 h1 (LSeq.create (2 * v (nlimbs l)) (limb_zero l)))
 
 
 inline_for_extraction noextract
-val create_point: unit -> StackInline point
+val create_point: l:limb_t -> StackInline (point l)
   (requires fun h -> True)
   (ensures  fun h0 f h1 ->
-    stack_allocated f h0 h1 (LSeq.create 12 (u64 0)))
+    stack_allocated f h0 h1 (LSeq.create (3 * v (nlimbs l)) (limb_zero l)))
 
 
-val make_base_point: p:point -> Stack unit
+val make_base_point: #l:limb_t -> p:point l -> Stack unit
   (requires fun h -> live h p)
   (ensures fun h0 _ h1 -> modifies (loc p) h0 h1 /\
-    point_inv h1 p /\ from_mont_point (as_point_nat h1 p) == S.base_point)
+    point_inv h1 p /\
+    from_mont_point (as_point_nat h1 p) == S.base_point)
 
 
-val make_point_at_inf: p:point -> Stack unit
+val make_point_at_inf: #l:limb_t -> p:point l -> Stack unit
   (requires fun h -> live h p)
   (ensures fun h0 _ h1 -> modifies (loc p) h0 h1 /\
     point_inv h1 p /\ from_mont_point (as_point_nat h1 p) == S.point_at_inf)
@@ -154,15 +155,15 @@ val make_point_at_inf: p:point -> Stack unit
 
 ///  Check if a point is a point-at-infinity
 
-val is_point_at_inf: p:point -> Stack uint64
+val is_point_at_inf: #l:limb_t -> p:point l -> Stack (limb l)
   (requires fun h -> live h p /\ point_inv h p)
   (ensures fun h0 r h1 -> modifies0 h0 h1 /\
     (let pM = from_mont_point (as_point_nat h0 p) in
-    (if S.is_point_at_inf pM then v r = ones_v U64 else v r = 0) /\
-    (if S.is_point_at_inf (as_point_nat h0 p) then v r = ones_v U64 else v r = 0)))
+    (if S.is_point_at_inf pM then v r = ones_v l else v r = 0) /\
+    (if S.is_point_at_inf (as_point_nat h0 p) then v r = ones_v l else v r = 0)))
 
 
-val is_point_at_inf_vartime: p:point -> Stack bool
+val is_point_at_inf_vartime: #l:limb_t -> p:point l -> Stack bool
   (requires fun h -> live h p /\ point_inv h p)
   (ensures  fun h0 r h1 -> modifies0 h0 h1 /\
     r == S.is_point_at_inf (as_point_nat h0 p) /\
@@ -172,7 +173,7 @@ val is_point_at_inf_vartime: p:point -> Stack bool
 ///  Create a copy of a point
 
 inline_for_extraction noextract
-val copy_point: res:point -> p:point -> Stack unit
+val copy_point: #l:limb_t -> res:point l -> p:point l -> Stack unit
   (requires fun h -> live h p /\ live h res /\ disjoint p res)
   (ensures fun h0 _ h1 -> modifies (loc res) h0 h1 /\
     as_seq h1 res == as_seq h0 p)
@@ -181,7 +182,7 @@ val copy_point: res:point -> p:point -> Stack unit
 ///  Point conversion between Projective and Affine coordinates representations
 
 // to_aff_point = S.to_aff_point + from_mont
-val to_aff_point: res:aff_point -> p:point -> Stack unit
+val to_aff_point: #l:limb_t -> res:aff_point l -> p:point l -> Stack unit
   (requires fun h ->
     live h p /\ live h res /\ eq_or_disjoint p res /\
     point_inv h p)
@@ -190,7 +191,7 @@ val to_aff_point: res:aff_point -> p:point -> Stack unit
 
 
 // to_aff_point = S.to_aff_point + from_mont
-val to_aff_point_x: res:felem -> p:point -> Stack unit
+val to_aff_point_x: #l:limb_t -> res:felem l -> p:point l -> Stack unit
   (requires fun h ->
     live h p /\ live h res /\ eq_or_disjoint p res /\
     point_inv h p)
@@ -199,7 +200,7 @@ val to_aff_point_x: res:felem -> p:point -> Stack unit
 
 
 // to_proj_point = S.to_proj_point + to_mont
-val to_proj_point: res:point -> p:aff_point -> Stack unit
+val to_proj_point: #l:limb_t -> res:point l -> p:aff_point l -> Stack unit
   (requires fun h ->
     live h p /\ live h res /\ disjoint p res /\
     aff_point_inv h p)
@@ -210,7 +211,7 @@ val to_proj_point: res:point -> p:aff_point -> Stack unit
 
 ///  Check if a point is on the curve
 
-val is_on_curve_vartime: p:aff_point -> Stack bool
+val is_on_curve_vartime: #l:limb_t -> p:aff_point l -> Stack bool
   (requires fun h -> live h p /\ aff_point_inv h p)
   (ensures fun h0 r h1 -> modifies0 h0 h1 /\
     r == S.is_on_curve (as_aff_point_nat h0 p))
@@ -218,7 +219,7 @@ val is_on_curve_vartime: p:aff_point -> Stack bool
 
 ///  Point load and store functions
 
-val aff_point_store: res:lbuffer uint8 64ul -> p:aff_point -> Stack unit
+val aff_point_store: #l:limb_t -> res:lbuffer uint8 64ul -> p:aff_point l -> Stack unit
   (requires fun h ->
     live h res /\ live h p /\ disjoint res p /\
     aff_point_inv h p)
@@ -226,7 +227,7 @@ val aff_point_store: res:lbuffer uint8 64ul -> p:aff_point -> Stack unit
     as_seq h1 res == S.aff_point_store (as_aff_point_nat h0 p))
 
 
-val point_store: res:lbuffer uint8 64ul -> p:point -> Stack unit
+val point_store: #l:limb_t -> res:lbuffer uint8 64ul -> p:point l -> Stack unit
   (requires fun h ->
     live h res /\ live h p /\ disjoint res p /\
     point_inv h p)
@@ -234,7 +235,7 @@ val point_store: res:lbuffer uint8 64ul -> p:point -> Stack unit
     as_seq h1 res == S.point_store (from_mont_point (as_point_nat h0 p)))
 
 
-val aff_point_load_vartime: res:aff_point -> b:lbuffer uint8 64ul -> Stack bool
+val aff_point_load_vartime: #l:limb_t -> res:aff_point l -> b:lbuffer uint8 64ul -> Stack bool
   (requires fun h ->
     live h res /\ live h b /\ disjoint res b)
   (ensures  fun h0 r h1 -> modifies (loc res) h0 h1 /\
@@ -242,7 +243,7 @@ val aff_point_load_vartime: res:aff_point -> b:lbuffer uint8 64ul -> Stack bool
     (r <==> Some? ps) /\ (r ==> (aff_point_inv h1 res /\ as_aff_point_nat h1 res == Some?.v ps))))
 
 
-val load_point_vartime: res:point -> b:lbuffer uint8 64ul -> Stack bool
+val load_point_vartime: #l:limb_t -> res:point l -> b:lbuffer uint8 64ul -> Stack bool
   (requires fun h ->
     live h res /\ live h b /\ disjoint res b)
   (ensures  fun h0 r h1 -> modifies (loc res) h0 h1 /\
@@ -251,7 +252,7 @@ val load_point_vartime: res:point -> b:lbuffer uint8 64ul -> Stack bool
       from_mont_point (as_point_nat h1 res) == Some?.v ps))))
 
 
-val aff_point_decompress_vartime (x y:felem) (s:lbuffer uint8 33ul) : Stack bool
+val aff_point_decompress_vartime (#l:limb_t) (x y:felem l) (s:lbuffer uint8 33ul) : Stack bool
   (requires fun h ->
     live h x /\ live h y /\ live h s /\
     disjoint x y /\ disjoint x s /\ disjoint y s)
