code/ecdsap256/Hacl.Impl.P256.PointDouble.fsti
@@ -7,13 +7,14 @@ module ST = FStar.HyperStack.ST
 open Lib.IntTypes
 open Lib.Buffer
 
+open Hacl.Impl.P256.Bignum
 open Hacl.Impl.P256.Point
 
 module S = Spec.P256
 
 #set-options "--z3rlimit 30 --fuel 0 --ifuel 0"
 
-val point_double: res:point -> p:point -> Stack unit
+val point_double: #l:limb_t -> res:point l -> p:point l -> Stack unit
   (requires fun h ->
     live h p /\ live h res /\ eq_or_disjoint p res /\
     point_inv h p)
